added `Seq.Satisfies` module and improved `Seq.Find` module.

src/spec/Flutterbye.Seq.Mem.fst
@@ -18,15 +18,19 @@
 
 module Flutterbye.Seq.Mem
 open FStar.Seq
-open Flutterbye.Seq.Find
+open Flutterbye.Seq.Satisfies
 
 type mem_p (#a_t:Type) (a:a_t) (s:seq a_t) =
    (exists (x:nat).
       x < length s && index s x = a)
 
+private val eq: 'a -> 'a -> Tot bool
+let eq a_1 a_2 =
+   a_1 = a_2
+
 val mem: x:'a -> s:seq 'a -> Tot (b:bool{b <==> mem_p x s})
 let mem a s =
-   is_Some (find (fun a' -> a = a') s)
+   satisfies (eq a) s
 
 abstract val index_lemma:
    s:seq 'a ->
@@ -37,7 +41,7 @@ abstract val index_lemma:
             (forall (x:nat).
                x < length s ==> mem_p (index s x) s)))
 let index_lemma s =
-   ()
+   Flutterbye.Seq.Satisfies.index_lemma s
 
 abstract val slice_lemma:
    s:seq 'a ->
@@ -50,7 +54,7 @@ abstract val slice_lemma:
                (forall z.
                   mem_p z (slice s x y) ==> mem_p z s)))
 let slice_lemma s =
-   ()
+   Flutterbye.Seq.Satisfies.slice_lemma s
 
 private type empty_p (#a_t:Type) (s:seq a_t) =
    forall (x:a_t).
@@ -60,11 +64,7 @@ abstract val empty_lemma:
    s:seq 'a ->
    Lemma (ensures (length s = 0 <==> empty_p s))
 let empty_lemma s =
-   if length s = 0 then
-      ()
-   else
-      (assert (mem_p (index s 0) s); // required witness
-      assert (~ (empty_p s)))
+   Flutterbye.Seq.Satisfies.empty_lemma s
 
 abstract val create_lemma:
    n:nat ->
@@ -76,23 +76,22 @@ abstract val create_lemma:
          // otherwise, only `a` can be a member of the resulting sequence.
          (n > 0 <==> mem_p a (create n a))))
 let create_lemma n a =
-   if n = 0 then
-      ()
-   else
-      let s = create n a in
-      assert (index s 0 = a) // required witness
+   Flutterbye.Seq.Satisfies.create_lemma n a
 
 abstract val append_lemma:
-   s_1:seq 'a ->
-   s_2:seq 'a ->
-   Lemma
+      #a_t:Type
+   -> s_1:seq a_t
+   -> s_2:seq a_t
+   -> Lemma
       (ensures
-         (forall x.
-            mem_p x s_1 ==> mem_p x (append s_1 s_2))
-         \/ (forall x.
-               mem_p x s_2 ==> mem_p x (append s_1 s_2))
-         // the following clause isn't successfully proven without the previous two.
-         \/ (forall x.
-            mem_p x (append s_1 s_2) <==> (mem_p x s_1 \/ mem_p x s_2)))
-let append_lemma s_1 s_2 =
-   ()
+         (  (forall (a:a_t).
+               mem_p a s_1 ==> mem_p a (append s_1 s_2))
+         \/ (forall (a:a_t).
+               mem_p a s_2 ==> mem_p a (append s_1 s_2))
+            // the following clause isn't successfully proven without the previous two.
+         \/ (forall (a:a_t).
+               mem_p a (append s_1 s_2) <==> (mem_p a s_1 \/ mem_p a s_2))
+         )      
+      )
+let append_lemma #a_t s_1 s_2 =
+   Flutterbye.Seq.Satisfies.append_lemma s_1 s_2
